Misc lemmas and cleanup

LTS.v
@@ -62,28 +62,6 @@ Section LTS.
 Context {lts : LTS}.
 Context (delay : SimOpt.delay_opt).
 
-#[global] Instance :
-  Proper (weq ==> eq ==> eq ==> iff) (hrel_of (n := lts.(St)) (m := lts.(St))).
-Proof.
-  cbn. intros. subst. apply H.
-Qed.
-
-#[global] Instance : Proper (leq ==> eq ==> eq ==> impl) (hrel_of (n := lts.(St)) (m := lts.(St))).
-Proof.
-  cbn. intros. subst. now apply H.
-Qed.
-
-#[global] Instance :
-  Proper (weq ==> eq ==> eq ==> iff) (hrel_of (n := lts.(St)) (m := lts.(St))).
-Proof.
-  cbn. intros. subst. apply H.
-Qed.
-
-#[global] Instance : Proper (leq ==> eq ==> eq ==> impl) (hrel_of (n := lts.(St)) (m := lts.(St))).
-Proof.
-  cbn. intros. subst. now apply H.
-Qed.
-
 Definition is_obs (l : @label lts.(Observable)) := if l then true else false.
 Definition is_tau (l : @label lts.(Observable)) := if l then false else true.
 
@@ -208,7 +186,90 @@ Proof.
   now rewrite <- str_refl, dot1x.
 Qed.
 
+Lemma dtrans_case : forall l st st',
+  dtrans l st st' ->
+  trans l st st' \/
+  (delay = SimOpt.delay /\ ((trans tau)^+ ⋅ trans l) st st').
+Proof.
+  intros. red in H. destruct delay.
+  - rewrite str_itr, dotplsx, dot1x in H. destruct H.
+    + now left.
+    + now right.
+  - now left.
+Qed.
+
+Lemma dtrans_tauplus : forall s s',
+  dtrans tau s s' ->
+  (lts.(trans) tau)^+ s s'.
+Proof.
+  intros. apply dtrans_trans in H. now rewrite <- itr_str_r in H.
+Qed.
+
+
+(* Epsilon *)
+
+Definition epsilon s s' := forall l t, lts.(trans) l s' t -> trans l s t.
+
+#[export] Instance epsilon_Eq : Proper (lts.(St).(Eq) ==> lts.(St).(Eq) ==> impl) epsilon.
+Proof.
+  cbn. red. intros.
+  rewrite <- H. rewrite <- H0 in H2. now apply H1.
+Qed.
+
+Lemma epsilon_plus : forall l s s' t,
+  epsilon s s' ->
+  (trans l)^+ s' t ->
+  (trans l)^+ s t.
+Proof.
+  intros. rewrite itr_str_l in H0 |- *.
+  destruct H0. apply H in H0.
+  esplit; eauto.
+Qed.
+
+Lemma epsilon_dtrans : forall l s s' t,
+  epsilon s s' ->
+  dtrans l s' t ->
+  dtrans l s t.
+Proof.
+  intros. apply dtrans_case in H0 as [].
+  - apply H in H0. now apply trans_dtrans.
+  - red. destruct H0 as [-> ?].
+    rewrite <- str_itr'.
+    rewrite itr_str_l, <- dotA in H0 |- *. destruct H0.
+    esplit; eauto.
+Qed.
+
+Lemma epsilon_is_stuck : forall s s',
+  epsilon s s' ->
+  is_stuck s ->
+  is_stuck s'.
+Proof.
+  intros ?????. apply H0. destruct H1.
+  apply H in H1. econstructor; eauto.
+Qed.
+
+Lemma epsilon_can_be_stuck : forall s s',
+  epsilon s s' ->
+  extrans s' ->
+  can_be_stuck s' ->
+  can_be_stuck s.
+Proof.
+  intros ?????. red. destruct H1 as [| (-> & ? & ? & ?)].
+  - now apply H1 in H0.
+  - right. split; auto.
+    rewrite str_itr in H1. destruct H1.
+    + cbn in H1. rewrite H1 in H0. now apply H2 in H0.
+    + eapply epsilon_plus in H1; eauto.
+      exists x. split; auto. now rewrite <- str_itr'.
+Qed.
+
 End LTS.
+
+Lemma tauplus_dtrans {lts} : forall s s',
+  (lts.(trans) tau)^+ s s' -> dtrans SimOpt.delay tau s s'.
+Proof.
+  intros. red. now rewrite <- itr_str_r.
+Qed.
 
 Hint Resolve is_tau_state_obs : optsim.
 Hint Resolve is_obs_state_tau : optsim.
